Organize inverses and related operational classes.

fowl/Is/OneSortedGroup.v
@@ -1,24 +1,24 @@
+(** * Group *)
+
 From Maniunfold.Has Require Export
   BinaryOperation NullaryOperation
   UnaryOperation.
 From Maniunfold.Is Require Export
-  Monoid OneSortedInvertible
+  Monoid Invertible
   OneSortedCancellative OneSortedUnaryAntidistributive Injective
   OneSortedInvolutive OneSortedUnaryAbsorbing.
 From Maniunfold.ShouldHave Require Import
   AdditiveNotations.
 
-(** * Group *)
-
 Class IsGrp (A : Type)
-  (Hk : HasBinOp A) (Hx : HasNullOp A) (Hf : HasUnOp A) : Prop := {
+  (Hx : HasNullOp A) (Hf : HasUnOp A) (Hk : HasBinOp A) : Prop := {
   is_mon :> IsMon 0 _+_;
-  is_inv_l_r :> IsInvLR bin_op null_op un_op;
+  is_inv_l_r :> IsInvLR 0 -_ _+_;
 }.
 
 Section Context.
 
-Context (A : Type) `{IsGrp A}.
+Context (A : Type) `(IsGrp A).
 
 (** TODO If we use section notations here,
     the following `Let` becomes useless. *)
@@ -28,11 +28,11 @@ Let bin_op : HasBinOp A := bin_op.
 Theorem bin_op_l_cancel (x y z : A) (e : z + x = z + y) : x = y.
 Proof.
   rewrite <- (unl_bin_op_l x).
-  rewrite <- (l_inv z).
+  rewrite <- (inv_l z).
   rewrite <- (assoc (- z) z x).
   rewrite e.
   rewrite (assoc (- z) z y).
-  rewrite (l_inv z).
+  rewrite (inv_l z).
   rewrite (unl_bin_op_l y).
   reflexivity. Qed.
 
@@ -42,11 +42,11 @@ Proof. exact @bin_op_l_cancel. Qed.
 Theorem bin_op_r_cancel (x y z : A) (e : x + z = y + z) : x = y.
 Proof.
   rewrite <- (unl_bin_op_r x).
-  rewrite <- (r_inv z).
+  rewrite <- (inv_r z).
   rewrite (assoc x z (- z)).
   rewrite e.
   rewrite <- (assoc y z (- z)).
-  rewrite (r_inv z).
+  rewrite (inv_r z).
   rewrite (unl_bin_op_r y).
   reflexivity. Qed.
 
@@ -59,12 +59,12 @@ Proof. split; typeclasses eauto. Qed.
 Theorem bin_op_un_op_un_antidistr (x y : A) : - (x + y) = (- y) + (- x).
 Proof.
   apply (l_cancel (- (x + y)) ((- y) + (- x)) (x + y)).
-  rewrite (r_inv (x + y)).
+  rewrite (inv_r (x + y)).
   rewrite (assoc (x + y) (- y) (- x)).
   rewrite <- (assoc x y (- y)).
-  rewrite (r_inv y).
+  rewrite (inv_r y).
   rewrite (unl_bin_op_r x).
-  rewrite (r_inv x).
+  rewrite (inv_r x).
   reflexivity. Qed.
 
 Global Instance bin_op_un_op_is_un_antidistr : IsUnAntidistr bin_op un_op.
@@ -73,10 +73,10 @@ Proof. exact @bin_op_un_op_un_antidistr. Qed.
 Theorem un_op_inj (x y : A) (e : - x = - y) : x = y.
 Proof.
   rewrite <- (unl_bin_op_l y).
-  rewrite <- (r_inv x).
+  rewrite <- (inv_r x).
   rewrite e.
   rewrite <- (assoc x (- y) y).
-  rewrite (l_inv y).
+  rewrite (inv_l y).
   rewrite (unl_bin_op_r x).
   reflexivity. Qed.
 
@@ -86,9 +86,9 @@ Proof. exact @un_op_inj. Qed.
 Theorem un_op_invol (x : A) : - (- x) = x.
 Proof.
   rewrite <- (unl_bin_op_r (- (- x))).
-  rewrite <- (l_inv x).
+  rewrite <- (inv_l x).
   rewrite (assoc (- (- x)) (- x) x).
-  rewrite (l_inv (- x)).
+  rewrite (inv_l (- x)).
   rewrite (unl_bin_op_l x).
   reflexivity. Qed.
 
@@ -98,7 +98,7 @@ Proof. exact @un_op_invol. Qed.
 Theorem null_op_un_op_un_absorb : - 0 = 0.
 Proof.
   rewrite <- (unl_bin_op_r (- 0)).
-  rewrite (l_inv 0).
+  rewrite (inv_l 0).
   reflexivity. Qed.
 
 Global Instance null_op_un_op_is_un_absorb : IsUnAbsorb null_op un_op.
