fowl/Is/CategoricalGroupoid.v
@@ -9,7 +9,7 @@ From Maniunfold.ShouldHave Require Import
 Class IsGrpd (A : Type)
   `(HasHom A) `(!HasCompHom hom) `(!HasIdHom hom) `(!HasInvHom hom) : Prop := {
   comp_hom_id_hom_is_cat :> IsCat comp_hom id_hom;
-  comp_hom_id_hom_inv_hom_is_cat_inv_hom :> IsCatInv comp_hom id_hom inv_hom;
+  comp_hom_id_hom_inv_hom_is_cat_inv_hom :> IsCatInvLR id_hom inv_hom comp_hom;
 }.
 
 Section Context.
@@ -19,9 +19,9 @@ Context (A : Type) `{IsGrpd A}.
 Theorem inv_hom_cat_invol (x y : A) (f : x --> y) : (f ^-1) ^-1 = f.
 Proof.
   rewrite <- (cat_unl_r _ _ ((f ^-1) ^-1)).
-  rewrite <- (cat_l_inv_hom _ _ f).
+  rewrite <- (cat_inv_l _ _ f).
   rewrite (cat_assoc _ _ _ _ ((f ^-1) ^-1) (f ^-1) f).
-  rewrite (cat_l_inv_hom _ _ (f ^-1)).
+  rewrite (cat_inv_l _ _ (f ^-1)).
   rewrite (cat_unl_l _ _ f).
   reflexivity. Qed.
 
