fowl/Is/CategoricalLeftInvertible.v
@@ -1,9 +1,0 @@
-From Maniunfold.Has Require Export
-  Morphism ComposedMorphism
-  IdentityMorphism InverseMorphism.
-From Maniunfold.ShouldHave Require Import
-  CategoricalNotations.
-
-Class IsCatLInv (A : Type) `(HasHom A)
-  `(!HasCompHom hom) `(!HasIdHom hom) `(!HasInvHom hom) : Prop :=
-  cat_l_inv_hom : forall (x y : A) (f : x --> y), f o f ^-1 = id.
