fowl/Is/Invertible.v
@@ -1,0 +1,20 @@
+(** * Invertibility of a Unary Operation with respect to a Binary Operation *)
+
+From Maniunfold.Has Require Export
+  NullaryOperation UnaryOperation BinaryOperation.
+From Maniunfold.ShouldHave Require Import
+  OneSortedAdditiveNotations.
+
+Class IsInvL (A : Type)
+  (Hx : HasNullOp A) (Hf : HasUnOp A) (Hk : HasBinOp A) : Prop :=
+  inv_l (x : A) : (- x) + x = 0.
+
+Class IsInvR (A : Type)
+  (Hx : HasNullOp A) (Hf : HasUnOp A) (Hk : HasBinOp A) : Prop :=
+  inv_r (x : A) : x + (- x) = 0.
+
+Class IsInvLR (A : Type)
+  (Hx : HasNullOp A) (Hf : HasUnOp A) (Hk : HasBinOp A) : Prop := {
+  is_inv_l :> IsInvL 0 -_ _+_;
+  is_inv_r :> IsInvR 0 -_ _+_;
+}.
