fowl/Is/TwoSortedLeftGroupAction.v
@@ -8,6 +8,6 @@ From Maniunfold.Is Require Export
 Class IsLGrpAct (A B : Type)
   `(HasBinOp A) `(HasNullOp A)
   `(HasUnOp A) `(HasActL A B) : Prop := {
-  A_bin_op_null_op_un_op_is_grp :> IsGrp bin_op null_op un_op;
+  A_bin_op_null_op_un_op_is_grp :> IsGrp null_op un_op bin_op;
   A_B_bin_op_null_op_act_l_is_l_mon_act :> IsLMonAct bin_op null_op act_l;
 }.
