fowl/Provides/ZTheorems.v
@@ -43,18 +43,18 @@ Proof. split; typeclasses eauto. Defined.
 Global Instance Z_bin_op_null_op_is_comm_mon : IsCommMon (bin_op (A := Z)) null_op.
 Proof. split; typeclasses eauto. Defined.
 
-Global Instance Z_bin_op_null_op_un_op_is_l_inv_hom :
-  IsLInv (bin_op (A := Z)) null_op un_op.
+Global Instance Z_bin_op_null_op_un_op_is_inv_l_hom :
+  IsInvL null_op un_op (bin_op (A := Z)).
 Proof. intros x. apply Z.add_opp_diag_l. Defined.
 
-Global Instance Z_bin_op_null_op_un_op_is_r_inv_hom :
-  IsRInv (bin_op (A := Z)) null_op un_op.
+Global Instance Z_bin_op_null_op_un_op_is_inv_r_hom :
+  IsInvR null_op un_op (bin_op (A := Z)).
 Proof. intros x. apply Z.add_opp_diag_r. Defined.
 
-Global Instance Z_bin_op_null_op_un_op_is_inv_hom : IsInvLR (bin_op (A := Z)) null_op un_op.
+Global Instance Z_bin_op_null_op_un_op_is_inv_hom : IsInvLR null_op un_op (bin_op (A := Z)).
 Proof. split; typeclasses eauto. Defined.
 
-Global Instance Z_bin_op_null_op_un_op_is_grp : IsGrp (bin_op (A := Z)) null_op un_op.
+Global Instance Z_bin_op_null_op_un_op_is_grp : IsGrp null_op un_op (bin_op (A := Z)).
 Proof. split; typeclasses eauto. Defined.
 
 Global Instance Z_bin_op_null_op_un_op_is_ab_grp :
