fowl/ShouldOffer/OneSortedMultiplicativeIntegerOperationNotations.v
@@ -3,5 +3,5 @@ From Maniunfold.Offers Require Import
 From Maniunfold.ShouldHave Require Export
   OneSortedMultiplicativeNotations.
 
-Notation "'_^_'" := (z_op bin_op null_op un_op) : Z_scope.
-Notation "x '^' n" := (z_op bin_op null_op un_op n x) : Z_scope.
+Notation "'_^_'" := (z_op null_op un_op bin_op) : Z_scope.
+Notation "x '^' n" := (z_op null_op un_op bin_op n x) : Z_scope.
